Aoc2025/Day04.lean
@@ -1,4 +1,5 @@
 import Aoc2025.Util
+import Std.Data.HashMap
 
 namespace Day04
 open Day04
@@ -23,29 +24,61 @@ def parseInput : IO (Grid Cell) := do
   let stdin <- IO.getStdin
   Grid.fromLines (<- stdin.lines) Cell.parse
 
+abbrev IsRoll (grid : Grid Cell) (pos : Coord) :=
+  grid[pos]? = some Cell.roll
+abbrev accessibility (grid : Grid Cell) (pos : Coord) :=
+  pos.adjacent.countP (IsRoll grid ·)
 abbrev ForkLiftAccessible (grid : Grid Cell) (pos : Coord) :=
-  pos.adjacent.countP (grid[·]? = some Cell.roll) < 4
+  accessibility grid pos < 4
 
-def getForkliftAccessible (grid : Grid Cell) : Array Coord := Id.run do
-  let mut ret := #[]
+structure AccessibilityMap where
+  grid : Grid Cell
+  accessibleCoords : Array { pos : Coord // ForkLiftAccessible grid pos }
+  coordToAcc : Std.DHashMap Coord (fun pos =>
+    { n : Nat // n = accessibility grid pos })
+
+def Grid.removeTowel (grid : Grid Cell) (pos : Coord) : Grid Cell :=
+  grid.set? pos .nil
+
+def AccessibilityMap.get (grid : Grid Cell) : AccessibilityMap := Id.run do
+  let mut accessible := #[]
+  let mut coordMap := Std.DHashMap.emptyWithCapacity
   for y in List.range grid.height do
     for x in List.range grid.width do
-      if grid[Coord.mk x y]? = some .roll ∧ ForkLiftAccessible grid ⟨x, y⟩
-      then ret := ret.push ⟨x, y⟩
-  return ret
+      let pos := Coord.mk x y
+      if IsRoll grid pos then
+        let acc := accessibility grid pos
+        if h : acc < 4
+        then accessible := accessible.push ⟨pos, by grind⟩
+        else coordMap := coordMap.insert pos ⟨acc, by rfl⟩
+  return ⟨grid, accessible, coordMap⟩
 
-def part1 (grid : Grid Cell) : IO Nat := do
-  return (getForkliftAccessible grid).size
+def part1 (grid : Grid Cell) : Id Nat := do
+  let acc := AccessibilityMap.get grid
+  return acc.accessibleCoords.size
 
-def part2 (grid : Grid Cell) : IO Nat := do
-  let mut grid := grid
+def part2 (grid : Grid Cell) : Id Nat := do
   let mut total := 0
+  let accMap := AccessibilityMap.get grid
+  -- It would be nice to have the queue and cache retain their
+  -- dependent types that prove their correspondence to the grid
+  -- state, but it would be too much effort to prove.
+  let mut grid := accMap.grid
+  let mut queue := accMap.accessibleCoords.map (fun pos => pos.1)
+  let mut coordToAcc := Std.HashMap.mk <| accMap.coordToAcc.map (fun _ v => v.1)
   for _ in List.range (grid.width * grid.height) do
-    let accessible := getForkliftAccessible grid
-    if accessible = #[] then break
-    total := total + accessible.size
-    for pos in accessible do
-      grid := grid.set? pos .nil
+    if h : queue.size = 0 then break else
+    let pos := queue.back
+    queue := queue.pop
+    total := total + 1
+    grid := grid.removeTowel pos
+    for pos' in pos.adjacent do
+      if h : IsRoll grid pos' ∧ pos' ∈ coordToAcc then
+        let acc := coordToAcc[pos']'h.2
+        if hacc : acc = 4
+        then queue := queue.push pos'
+             coordToAcc := coordToAcc.erase pos'
+        else coordToAcc := coordToAcc.insert pos' (acc - 1)
   return total
 
 end Day04
